silveroak-opentitan/hmac/end2end/Sha256ToCava.v
@@ -3,82 +3,177 @@ Require Import Coq.ZArith.ZArith. Open Scope Z_scope.
 Require Import Coq.Strings.String. Open Scope string_scope.
 Require Import coqutil.Byte.
 Require Import coqutil.Word.Interface coqutil.Word.Properties.
+Require Import coqutil.Tactics.fwd coqutil.Tactics.Tactics.
 Require Import bedrock2.ZnWords.
 Require Import compiler.SeparationLogic.
+Require Import compiler.LowerPipeline.
 Require Import Bedrock2Experiments.RiscvMachineWithCavaDevice.ExtraRiscvMachine.
 Require Import Bedrock2Experiments.RiscvMachineWithCavaDevice.InternalMMIOMachine.
 Require Import HmacEnd2End.CavaHmacDevice.
 Require Import HmacSoftware.Sha256ToRiscV.
+Require Import HmacSpec.SHA256.
 Require Import Bedrock2Experiments.RiscvMachineWithCavaDevice.Bedrock2ToCava.
 
 Definition binary: list byte := Eval compute in Pipeline.instrencode sha256_asm.
 
-(* TODO replace axiom from HmacSemantics with actual spec *)
-Definition sha256 := HmacSemantics.sha256.
+(* TODO: replace by actual hmac device init state *)
+Definition IDLE: unit := tt.
 
-Axiom TODO: False.
+Definition machine_valid(imem: mem -> Prop)(mach: ExtraRiscvMachine hmac_device): Prop :=
+  subset (footpr imem) (of_list (getXAddrs mach)) /\
+  getNextPc mach = word.add (getPc mach) (word.of_Z 4) /\
+  regs_initialized (getRegs mach) /\
+  map.undef_on (getMem mach) device.isMMIOAddr /\
+  disjoint (of_list (getXAddrs mach)) device.isMMIOAddr.
 
-Theorem sha256_example_end2end_correct: forall p_functions p_call mH Rdata Rexec R (* <-? *)
-          (initialL: ExtraRiscvMachine hmac_device) digest_addr input_addr input_len
-          input output_placeholder sched,
-    -2^19 <= word.signed (word.sub p_functions p_call) < 2^19 ->
-    128 <= word.unsigned (word.sub stack_pastend stack_start) ->
-    word.unsigned (word.sub stack_pastend stack_start) mod 4 = 0 ->
-    word.unsigned p_functions mod 4 = 0 ->
-    word.unsigned p_call mod 4 = 0 ->
-    initialL.(getLog) = [] ->
-    machine_ok p_functions stack_start stack_pastend binary
-               mH Rdata Rexec initialL ->
-    Z.of_nat (length input) = word.unsigned input_len ->
-    Z.of_nat (length output_placeholder) = 32 ->
-    input_addr <> word.of_Z 0 ->
-    digest_addr <> word.of_Z 0 ->
-    (bytearray input_addr input * bytearray digest_addr output_placeholder * R)%sep mH ->
-    exists steps_remaining finalL mH',
-      run sched steps_remaining initialL = (Some tt, finalL) /\
-      machine_ok p_functions stack_start stack_pastend binary
-                 mH' Rdata Rexec finalL /\
-    (bytearray input_addr input * bytearray digest_addr (sha256 input) * R)%sep mH' /\
-      finalL.(getLog) = initialL.(getLog) (* no external interactions happened *).
+Local Notation "a * b" := (sep a b) : type_scope.
+Local Notation "a * b" := (sep a b).
+
+Add Ring wring : (Properties.word.ring_theory (word := word))
+                   (preprocess [autorewrite with rew_word_morphism],
+                    morphism (Properties.word.ring_morph (word := word)),
+                    constants [Properties.word_cst]).
+
+Declare Scope word_scope.
+Infix "+" := word.add : word_scope.
+Infix "-" := word.sub : word_scope.
+Delimit Scope word_scope with word.
+Local Open Scope word_scope.
+
+Implicit Type m : ExtraRiscvMachine hmac_device.
+
+(* Trying to keep toplevel theorem at 53 chars wide:
+01234567890123456789012345678901234567890123456789012 *)
+
+Axiom sha256_len: forall inp, List.length (sha256 inp) = 32%nat.
+
+Theorem sha256_end2end_correct:
+  forall a_inp a_outp len inp p_code sp_val
+    stack_low_end ret_addr Rdata Rexec sched m,
+  Z.of_nat (length inp) = word.unsigned len ->
+  a_inp <> word.of_Z 0 ->
+  a_outp <> word.of_Z 0 ->
+  map.get m.(getRegs) RegisterNames.a0 = Some a_outp ->
+  map.get m.(getRegs) RegisterNames.a1 = Some a_inp ->
+  map.get m.(getRegs) RegisterNames.a2 = Some len ->
+  map.get m.(getRegs) RegisterNames.sp = Some sp_val ->
+  map.get m.(getRegs) RegisterNames.ra = Some ret_addr ->
+  m.(getPc) = p_code + word.of_Z sha256_relative_pos ->
+  256 <= word.unsigned (sp_val - stack_low_end) ->
+  word.unsigned (sp_val - stack_low_end) mod 4 = 0 ->
+  word.unsigned p_code mod 4 = 0 ->
+  word.unsigned ret_addr mod 4 = 0 ->
+  m.(getExtraState) = IDLE ->
+  machine_valid (ptsto_bytes p_code binary * Rexec) m ->
+  (bytearray a_inp inp *
+   mem_available a_outp (a_outp + (word.of_Z 32)) *
+   mem_available stack_low_end sp_val * Rdata *
+   ptsto_bytes p_code binary * Rexec) m.(getMem) ->
+  exists n m',
+  run sched n m = Some m' /\
+  map.get m'.(getRegs) RegisterNames.sp = Some sp_val /\
+  map.agree_on callee_saved m.(getRegs) m'.(getRegs) /\
+  m'.(getPc) = ret_addr /\
+  m'.(getExtraState) = IDLE /\
+  machine_valid (ptsto_bytes p_code binary * Rexec) m' /\
+  (bytearray a_inp inp *
+   bytearray a_outp (sha256 inp)  *
+   mem_available stack_low_end sp_val * Rdata *
+   ptsto_bytes p_code binary * Rexec) m'.(getMem).
 Proof.
   intros.
   change binary with (Pipeline.instrencode sha256_asm).
-Abort.
-(*
-  refine (bedrock2_and_cava_system_correct
-            _ _ _ _ _ _ _ _ _ _ _ _ _ _ _ _ _ _ _ _ _ _ _ _ _ _ _ _ _ _ _ _ _);
-    try eassumption.
+  assert (((mem_available a_outp (a_outp + (word.of_Z 32)) * bytearray a_inp inp) *
+           (mem_available stack_low_end sp_val * ptsto_bytes p_code binary * Rexec * Rdata))
+            m.(getMem)) as M by ecancel_assumption.
+  unfold sep in M at 1. destruct M as (mH & mL & Sp & MH & ML).
+  eapply mem_available_to_exists in MH.
+  destruct MH as (output_placeholder & HLen & MH).
+  ring_simplify (a_outp + word.of_Z 32 - a_outp) in HLen.
+  edestruct bedrock2_and_cava_system_correct with
+      (f_entry_name := "b2_sha256")
+      (stack_start := stack_low_end) (stack_pastend := sp_val)
+      (postH := fun mH' (retvals: list word) =>
+                  (bytearray a_inp inp * bytearray a_outp (sha256 inp)) mH')
+    as (steps_remaining & finalL & mH' & retvals & Rn & GM & A & Eq & M & HP);
+    lazymatch goal with
+    | |- _ mod _ = _ => idtac
+    | |- _ => try eassumption
+    end.
   { exact funcs_valid. }
-  { apply List.dedup_NoDup_iff with (aeqb_spec:=String.eqb_spec). reflexivity. }
+  { apply List.dedup_NoDup_iff. reflexivity. }
   { exact sha256_compile_result_eq. }
   { (* check that the compiler emitted valid instructions: *)
     repeat (apply Forall_cons || apply Forall_nil).
     all: try (vm_compute; intuition discriminate). }
-  { let p := eval cbv in main_relative_pos in change main_relative_pos with p. Lia.lia. }
-  { instantiate (2 := "main"). reflexivity. }
   { reflexivity. }
-  { vm_compute. discriminate. }
-  { refine (WeakestPreconditionProperties.Proper_cmd _ _ _ _ _ _ _ _ _ _ _).
-    1: eapply WeakestPreconditionProperties.Proper_call.
-    2: {
-      eapply main_correct with (idlebuffer := List.repeat Byte.x00 32); cycle -2; try eassumption.
-      match goal with
-      | H: ?t = ?t' |- _ ?t'' _ => replace t'' with t' by exact H
+  { change sha256_req_stack with (sha256_req_stack * 4 / 4).
+    eapply Z.div_le_mono. 1: reflexivity.
+    etransitivity. 2: eassumption.
+    vm_compute. discriminate. }
+  { assumption. }
+  { assumption. }
+  { assumption. }
+  { eapply WeakestPreconditionProperties.Proper_call.
+    2: eapply link_sha256.
+    6: { instantiate (4 := a_outp). instantiate (5 := a_inp). instantiate (1 := mH).
+         unfold ptsto_bytes in *. ecancel_assumption. }
+    6: { cbn. instantiate (1 := List.repeat Byte.x00 32). reflexivity. }
+    all: try eassumption.
+    unfold Morphisms.pointwise_relation, Basics.impl, Sha256ExampleProperties.sha256_post.
+    intros. fwd.
+    split. 1: ecancel_assumption.
+    eexists. split. 1: eassumption. cbn.
+    apply sha256_len. }
+  { cbn -[map.get].
+    repeat match goal with
+           | |- context[match ?x with _ => _ end] =>
+             match goal with
+             | H: ?x' = Some ?y |- _ => replace x with (Some y) by (symmetry; exact H)
+             end
+           end.
+    reflexivity. }
+  { unfold machine_ok, machine_valid in *. fwd.
+    unfold device.is_ready_state, hmac_device.
+    match goal with
+    | H: _ = IDLE |- _ => unfold IDLE in H; symmetry in H
+    end.
+    ssplit; try eassumption.
+    - change (Pipeline.instrencode sha256_asm) with binary.
+      apply sep_comm.
+      unfold sep at 1. exists mH, mL. split. 1: exact Sp. split. 1: reflexivity.
+      ecancel_assumption.
+    - match goal with
+      | |- word.unsigned ?x mod 4 = 0 => replace x with (p_code + word.of_Z sha256_relative_pos)
       end.
-      cbn.
-      case TODO.
-      (* make length of digest buffer match, and how to make it unique to satisfy Cava connection? *)
-    }
-    unfold Sha256ExampleProperties.sha256_post.
-    repeat intro. Tactics.logical_simplify. Tactics.ssplit.
-    { unfold sha256. ecancel_assumption. }
-    eexists. split; [eassumption|]. cbn. case TODO.
-    (* here, IDLE state with a sha in its digest_buffer must be an initial state *)
-  }
-  Unshelve. case TODO. (* initial state will be determined *)
+      let r := eval vm_compute in sha256_relative_pos in change sha256_relative_pos with r.
+      rewrite add_0_r. assumption. }
+  { unfold machine_ok in M. unfold machine_valid. fwd.
+    do 2 eexists. ssplit.
+    - unfold run. rewrite Rn. reflexivity.
+    - assumption.
+    - assumption.
+    - reflexivity.
+    - unfold device.is_ready_state, hmac_device, IDLE in *. symmetry. assumption.
+    - assumption.
+    - assumption.
+    - assumption.
+    - assumption.
+    - assumption.
+    - unfold sep at 1 in Mp0. destruct Mp0 as (mL' & mH'' & Sp' & ML' & ?).  subst mH''.
+      enough (((bytearray a_inp inp * bytearray a_outp (sha256 inp)) *
+              (mem_available stack_low_end sp_val * Rdata *
+               ptsto_bytes p_code (Pipeline.instrencode sha256_asm) * Rexec)) (getMem finalL))
+        by ecancel_assumption.
+      apply sep_comm.
+      unfold sep at 1.
+      exists mL', mH'. split. 1: exact Sp'. split. 2: exact HP.
+      ecancel_assumption. }
+  Unshelve.
+  all: repeat constructor.
+  all: try exact (word.of_Z 0).
 Qed.
-*)
 
 (* Goal: bring this list down to only standard axioms like functional and propositional extensionality
-Print Assumptions sha256_example_end2end_correct.
+Print Assumptions sha256_end2end_correct.
  *)
